CheriConfig.v
@@ -1,0 +1,223 @@
+Require Import Kami.AllNotations ProcKami.Lib ProcKami.CheriTypes.
+
+Definition CapStruct : Kind :=
+  (STRUCT_TYPE {
+       "R" :: Bit 1;
+       "p" :: Bit 6;
+       "oType" :: Bit 3;
+       "E" :: Bit 4;
+       "B" :: Bit 9;
+       "T" :: Bit 9 })%kami_expr.
+
+Section CapHelpers.
+  Section AddrSz.
+      Local Notation AddrSz := 32.
+    Section ty.
+      Variable ty: Kind -> Type.
+      Local Open Scope kami_expr.
+      Definition decodePerms (rawPerms: Array 6 Bool @# ty) :=
+        (IF rawPerms ![4]
+         then (IF rawPerms ![3]
+               then (STRUCT {
+                         "U0" ::= $$false;
+                         "SE" ::= $$false;
+                         "US" ::= $$false;
+                         "EX" ::= $$false;
+                         "SR" ::= $$false;
+                         "MC" ::= $$true;
+                         "LD" ::= $$true;
+                         "SL" ::= rawPerms ![2];
+                         "LM" ::= rawPerms ![1];
+                         "SD" ::= $$true;
+                         "LG" ::= rawPerms ![0];
+                         "GL" ::= rawPerms ![5] })
+               else (IF rawPerms ![2]
+                     then (STRUCT {
+                               "U0" ::= $$false;
+                               "SE" ::= $$false;
+                               "US" ::= $$false;
+                               "EX" ::= $$false;
+                               "SR" ::= $$false;
+                               "MC" ::= $$true;
+                               "LD" ::= $$true;
+                               "SL" ::= $$false;
+                               "LM" ::= rawPerms ![1];
+                               "SD" ::= $$false;
+                               "LG" ::= rawPerms ![0];
+                               "GL" ::= rawPerms ![5] })
+                     else (IF !(rawPerms ![1]) && !(rawPerms ![0])
+                           then (STRUCT {
+                                     "U0" ::= $$false;
+                                     "SE" ::= $$false;
+                                     "US" ::= $$false;
+                                     "EX" ::= $$false;
+                                     "SR" ::= $$false;
+                                     "MC" ::= $$true;
+                                     "LD" ::= $$false;
+                                     "SL" ::= $$false;
+                                     "LM" ::= $$false;
+                                     "SD" ::= $$true;
+                                     "LG" ::= $$false;
+                                     "GL" ::= rawPerms ![5] })
+                           else (STRUCT {
+                                     "U0" ::= $$false;
+                                     "SE" ::= $$false;
+                                     "US" ::= $$false;
+                                     "EX" ::= $$false;
+                                     "SR" ::= $$false;
+                                     "MC" ::= $$false;
+                                     "LD" ::= rawPerms ![1];
+                                     "SL" ::= $$false;
+                                     "LM" ::= $$false;
+                                     "SD" ::= rawPerms ![0];
+                                     "LG" ::= $$false;
+                                     "GL" ::= rawPerms ![5] }))))
+         else (IF rawPerms ![3]
+               then (STRUCT {
+                         "U0" ::= $$false;
+                         "SE" ::= $$false;
+                         "US" ::= $$false;
+                         "EX" ::= $$true;
+                         "SR" ::= rawPerms ![2];
+                         "MC" ::= $$true;
+                         "LD" ::= $$true;
+                         "SL" ::= $$false;
+                         "LM" ::= rawPerms ![1];
+                         "SD" ::= $$false;
+                         "LG" ::= rawPerms ![0];
+                         "GL" ::= rawPerms ![5] })
+               else (STRUCT {
+                         "U0" ::= rawPerms ![2];
+                         "SE" ::= rawPerms ![1];
+                         "US" ::= rawPerms ![0];
+                         "EX" ::= $$false;
+                         "SR" ::= $$false;
+                         "MC" ::= $$false;
+                         "LD" ::= $$false;
+                         "SL" ::= $$false;
+                         "LM" ::= $$false;
+                         "SD" ::= $$false;
+                         "LG" ::= $$false;
+                         "GL" ::= rawPerms ![5] }))).
+  
+      Definition encodePerms (perms: CapPerms @# ty) : Bit 6 @# ty :=
+        {< pack (perms @% "GL"),
+          ( IF perms @% "EX" && perms @% "LD" && perms @% "MC"
+            then {< Const ty (2'b"01"), pack (perms @% "SR"), pack (perms @% "LM"), pack (perms @% "LG") >}
+            else (IF perms @% "LD" && perms @% "MC" && perms @% "SD"
+                  then {< Const ty (2'b"11"), pack (perms @% "SL"), pack (perms @% "LM"), pack (perms @% "LG") >}
+                  else (IF perms @% "LD" && perms @% "MC"
+                        then {< Const ty (3'b"101"), pack (perms @% "LM"), pack (perms @% "LG") >}
+                        else (IF perms @% "SD" && perms @% "MC"
+                              then Const ty (5'b"10000")
+                              else (IF perms @% "LD" || perms @% "SD"
+                                    then {< Const ty (2'b"01"), pack (perms @% "SR"), pack (perms @% "LM"), pack (perms @% "LG") >}
+                                    else {< Const ty (2'b"00"), pack (perms @% "U0"), pack (perms @% "SE"), pack (perms @% "US") >})))))%kami_expr >}.
+  
+      Definition capExpFromE (E: Bit 4 @# ty) : Bit (Nat.log2_up AddrSz) @# ty :=  ITE (E == Const ty (wones _)) $24 (ZeroExtendTruncLsb _ E).
+  
+      Definition capBaseTop (cap: Bit (size CapStruct) @# ty) (addr: Bit AddrSz @# ty) :=
+        ( LETC B <- (unpack CapStruct cap) @% "B";
+          LETC T <- (unpack CapStruct cap) @% "T";
+          LETC E <- (unpack CapStruct cap) @% "E";
+          LETC exp <- capExpFromE #E;
+          LETC aMidTop <- addr >> #exp;
+          LETC aMid <- UniBit (TruncLsb 9 (AddrSz - 9)) #aMidTop;
+          LETC aTop <- UniBit (TruncMsb 9 (AddrSz - 9)) #aMidTop;
+          LETC aHi <- ITE (#aMid < #B) $1 $0;
+          LETC tHi <- ITE (#T < #B) $1 $0;
+          LETC aTopBase <- Sub #aTop #aHi;
+          LETC base <- ZeroExtendTruncLsb AddrSz ({< #aTopBase, #B >}) << #exp;
+          LETC top <- ZeroExtendTruncLsb (AddrSz + 1) ({< #aTopBase + #tHi, #T >}) << #exp;
+          RetE (STRUCT {
+                    "base" ::= #base;
+                    "top" ::= #top } : (STRUCT_TYPE { "base" :: Bit AddrSz ; "top" :: Bit (AddrSz + 1) }) @# ty) ).
+  
+      Definition capBounds (base: Bit AddrSz @# ty) (length: Bit AddrSz @# ty) :=
+        ( LETC top : Bit (AddrSz + 1) <- ZeroExtend 1 base + ZeroExtend 1 length;
+          LETC expInit : Bit (Nat.log2_up AddrSz) <- Sub $23 (countLeadingZeros _ (ZeroExtendTruncMsb 23 length));
+          LETC isInitSatExpInitSat : Pair Bool (Bit (Nat.log2_up AddrSz)) <-
+                                       ITE (#expInit > $14) (STRUCT { "fst" ::= $$true; "snd" ::= $$(wones 5) })
+                                         (STRUCT { "fst" ::= $$false; "snd" ::= #expInit });
+          LETC isInitSat <- #isInitSatExpInitSat @% "fst";
+          LETC expInitSat <- #isInitSatExpInitSat @% "snd";
+          LETC lostTopInit <- isNotZero (#top << (Sub $AddrSz #expInitSat));
+          LETC lengthShifted <- ZeroExtendTruncLsb 9 (length >> #expInitSat);
+          LETC lengthShiftedAllOnes <- isAllOnes #lengthShifted;
+          LETC exp : Bit (Nat.log2_up AddrSz) <- ITE (#lostTopInit && #lengthShiftedAllOnes && !#isInitSat)
+                                                   (#expInitSat + $1) (#expInitSat);
+          LETC B <- ZeroExtendTruncLsb 9 (base >> #exp);
+          LETC lostTop <- isNotZero (#top << (Sub $AddrSz #exp));
+          LETC TInit <- ZeroExtendTruncLsb 9 (#top >> #exp);
+          LETC T <- ITE #lostTop (#TInit + $1) #TInit;
+          LETC lostBase <- isNotZero (base << (Sub $AddrSz #exp));
+          RetE (STRUCT {
+                    "B" ::= #B;
+                    "T" ::= #T;
+                    "exp" ::= #exp;
+                    "exact?" ::= (#lostBase || #lostTop) } : STRUCT_TYPE { "B" :: Bit 9;
+                                                                           "T" :: Bit 9;
+                                                                           "exp" :: Bit (Nat.log2_up AddrSz);
+                                                                           "exact?" :: Bool } @# ty)).
+    End ty.
+  
+    Definition capAccessorsInit : CapAccessors _ _ :=
+      {|getCapR ty cap := (unpack CapStruct cap) @% "R";
+        setCapR ty val cap := pack ((unpack CapStruct cap) @%[ "R" <- val]);
+        getCapP ty cap := (unpack CapStruct cap) @% "p";
+        setCapP ty val cap := pack ((unpack CapStruct cap) @%[ "p" <- val]);
+        getCapOType ty cap := (unpack CapStruct cap) @% "oType";
+        setCapOType ty val cap := pack ((unpack CapStruct cap) @%[ "oType" <- val]);
+        getCapE ty cap := (unpack CapStruct cap) @% "E";
+        setCapE ty val cap := pack ((unpack CapStruct cap) @%[ "E" <- val]);
+        getCapB ty cap := (unpack CapStruct cap) @% "B";
+        setCapB ty val cap := pack ((unpack CapStruct cap) @%[ "B" <- val]);
+        getCapT ty cap := (unpack CapStruct cap) @% "T";
+        setCapT ty val cap := pack ((unpack CapStruct cap) @%[ "T" <- val]);
+        getCapEFromExp ty exp := ITE (exp >= Const ty (_ 'h"e")) $$(4'h"f") (ZeroExtendTruncLsb _ exp);
+        getCapExpFromE ty E := capExpFromE E;
+        isSealed t cap := (unpack CapStruct cap) @% "oType" != $0;
+        isSentry t cap := let oType := (unpack CapStruct cap) @% "oType" in (oType <= $3) && (oType >= $1);
+        isIeSentry t cap := (unpack CapStruct cap) @% "oType" == $2;
+        isIdSentry t cap := (unpack CapStruct cap) @% "oType" == $3;
+        getOTypeFromIe ty ie := ITE ie $2 $3;
+        seal ty val cap := pack ((unpack CapStruct cap) @%[ "oType" <- val]);
+        unseal ty cap := pack ((unpack CapStruct cap) @%[ "oType" <- $$(natToWord 3 0)]);
+        isSealAddr ty addr isExec := ITE isExec
+                                       (((addr >= $1) && (addr <= $3)) || addr == $6 || addr == $7)
+                                       ((addr >= $9) && (addr <= $15));
+        getCapPerms ty cap := (RetE decodePerms (unpack (Array 6 Bool) ((unpack CapStruct cap) @% "p")));
+        setCapPerms ty perms cap :=
+          ( LETC arr : Bit 6 <- encodePerms perms;
+            RetE (pack ((unpack CapStruct cap) @%[ "p" <- pack #arr ])) );
+        getCapBaseTop ty cap addr := capBaseTop cap addr;
+        getCapBounds ty base length := capBounds base length;
+      |}%kami_expr.
+
+    Definition PcCapInit := ((@wconcat 1 31 32 (1'b"0")
+                                (@wconcat 6 25 31 (6'b"101111")
+                                   (@wconcat 3 22 25 (3'h"0")
+                                      (@wconcat 4 18 22 (wones 4)
+                                         (@wconcat 9 9 18 (9'h"0")
+                                            (9'h"10")))))) : word AddrSz).
+    Definition PcAddrInit := (AddrSz 'h"1000").
+    
+    Theorem pccValidThm: PccValid capAccessorsInit PcCapInit PcAddrInit false.
+    Proof.
+      repeat constructor; auto.
+    Qed.
+  End AddrSz.
+End CapHelpers.
+
+Definition procParams : ProcParams :=
+  {|procName := "cheriot";
+    Xlen := 32;
+    xlenIs32_or_64 := or_introl eq_refl;
+    capAccessors := capAccessorsInit;
+    pccValid := pccValidThm;
+    TrapAddr := _ 'h"100";
+    supportedExts := [Base];
+    extsHasBase := or_introl eq_refl;
+    RegIdSz := 4;
+    regIdSzIs4_or5 := or_introl eq_refl
+  |}.
